Fix typing of reals, make typing tactic work for reals, and minor adjustments
Previously, the typing rules forced relational operators to be applicable only for integers. Now, the typing rules also permit reals (but never a mix of reals and integers, since such combinations are not well-typed in Boogie). Moreover, the typing rules are now expressed in a way that do not treat real division differently from integer division. As a result of this change, the typing tactic for real division should work (while previously it did not).

BoogieLang/Typing.thy
@@ -13,25 +13,24 @@ primrec unop_type :: "unop \<Rightarrow> prim_ty \<times> prim_ty"
     "unop_type UMinus = (TInt, TInt)"
   | "unop_type Not = (TBool, TBool)"
 
-primrec binop_type :: "binop \<Rightarrow> ((prim_ty \<times> prim_ty) \<times> prim_ty) option"
+primrec binop_type :: "binop \<Rightarrow> ((prim_ty \<times> prim_ty) set \<times> prim_ty) option"
   where
     "binop_type Eq = None"
   | "binop_type Neq = None"
-  \<comment>\<open>handle real division separately, since it allows multiple type combinations\<close>
-  | "binop_type RealDiv = None" 
-  | "binop_type Add = Some ((TInt, TInt), TInt)"
-  | "binop_type Sub = Some ((TInt, TInt), TInt)"
-  | "binop_type Mul = Some ((TInt, TInt), TInt)"
-  | "binop_type Div = Some ((TInt, TInt), TInt)"
-  | "binop_type Mod = Some ((TInt, TInt), TInt)"
-  | "binop_type Lt = Some ((TInt, TInt), TBool)"
-  | "binop_type Le = Some ((TInt, TInt), TBool)"
-  | "binop_type Gt = Some ((TInt, TInt), TBool)"
-  | "binop_type Ge = Some ((TInt, TInt), TBool)"
-  | "binop_type And = Some ((TBool, TBool), TBool)"
-  | "binop_type Or = Some ((TBool, TBool), TBool)"
-  | "binop_type Imp = Some ((TBool, TBool), TBool)"
-  | "binop_type Iff = Some ((TBool, TBool), TBool)"
+  | "binop_type RealDiv = Some ({(TInt, TInt), (TReal, TReal), (TInt, TReal), (TReal, TInt)}, TReal)" 
+  | "binop_type Add = Some ({(TInt, TInt)}, TInt)"
+  | "binop_type Sub = Some ({(TInt, TInt)}, TInt)"
+  | "binop_type Mul = Some ({(TInt, TInt)}, TInt)"
+  | "binop_type Div = Some ({(TInt, TInt)}, TInt)"
+  | "binop_type Mod = Some ({(TInt, TInt)}, TInt)"
+  | "binop_type Lt = Some ({(TInt, TInt), (TReal, TReal)}, TBool)"
+  | "binop_type Le = Some ({(TInt, TInt), (TReal, TReal)}, TBool)"
+  | "binop_type Gt = Some ({(TInt, TInt), (TReal, TReal)}, TBool)"
+  | "binop_type Ge = Some ({(TInt, TInt), (TReal, TReal)}, TBool)"
+  | "binop_type And = Some ({(TBool, TBool)}, TBool)"
+  | "binop_type Or = Some ({(TBool, TBool)}, TBool)"
+  | "binop_type Imp = Some ({(TBool, TBool)}, TBool)"
+  | "binop_type Iff = Some ({(TBool, TBool)}, TBool)"
 
 fun binop_poly_type :: "binop \<Rightarrow> bool"
   where 
@@ -47,15 +46,11 @@ and typing_list :: "fdecls \<Rightarrow> type_env \<Rightarrow> expr list \<Righ
   | TypBVar: "\<lbrakk> (snd \<Delta>) i = Some ty \<rbrakk> \<Longrightarrow> F,\<Delta> \<turnstile> BVar i : ty"
   | TypPrim: "\<lbrakk> type_of_lit l = prim_ty \<rbrakk> \<Longrightarrow> F,\<Delta> \<turnstile> Lit l : TPrim prim_ty"
   | TypUnOp: "\<lbrakk> unop_type uop = (arg_ty,ret_ty); F,\<Delta> \<turnstile> e : TPrim arg_ty\<rbrakk>   \<Longrightarrow> F,\<Delta> \<turnstile> UnOp uop e : TPrim ret_ty"
-  | TypBinOpMono: "\<lbrakk> binop_type bop = Some ((left_ty, right_ty), ret_ty); F,\<Delta> \<turnstile> e1 : TPrim left_ty; F,\<Delta> \<turnstile> e2 : TPrim right_ty \<rbrakk> \<Longrightarrow>
+  | TypBinOpMono: "\<lbrakk> binop_type bop = Some (targs, ret_ty); 
+                     F,\<Delta> \<turnstile> e1 : TPrim left_ty; 
+                     F,\<Delta> \<turnstile> e2 : TPrim right_ty;
+                     (left_ty, right_ty) \<in> targs  \<rbrakk> \<Longrightarrow>
                     F,\<Delta> \<turnstile> e1 \<guillemotleft>bop\<guillemotright> e2 : TPrim ret_ty"
-  | TypBinopRealDiv: 
-     "\<lbrakk> F,\<Delta> \<turnstile> e1 : TPrim t1; 
-        F,\<Delta> \<turnstile> e2 : TPrim t2; 
-        (t1 = TInt \<or> t1 = TReal);
-        (t2 = TInt \<or> t2 = TReal)
-      \<rbrakk> \<Longrightarrow>
-        F,\<Delta> \<turnstile> e1 \<guillemotleft>RealDiv\<guillemotright> e2 : TPrim TReal"
   (* equality and inequality are typed more liberally as also outlined in 
       This is Boogie (Leino) and
       A polymorphic intermediate verification language: Design and logical encoding (Leino and Ruemmer) *)
