BoogieLang/TypeSafety.thy
@@ -28,15 +28,17 @@ lemma unop_progress: "\<lbrakk> unop_type uop = (arg_ty, ret_ty); type_of_val A 
   by (cases uop; rule lit_val_elim[where v=v']; auto)
 
 lemma binop_type_correct: 
- "\<lbrakk> binop_type bop = Some ((left_ty,right_ty), ret_ty); 
+ "\<lbrakk> binop_type bop = Some (targs, ret_ty); 
     type_of_val  A v1 = (TPrim left_ty); type_of_val A v2 = (TPrim right_ty); 
+    (left_ty, right_ty) \<in> targs;
     (binop_eval_val bop v1 v2) = Some v  \<rbrakk> \<Longrightarrow>
     type_of_val A v = TPrim ret_ty"
   by (cases bop; rule lit_val_elim[where v=v1]; rule lit_val_elim[where v=v2]; auto)
 
 lemma binop_progress:
- "\<lbrakk> binop_type bop = Some ((left_ty,right_ty), ret_ty); 
-    type_of_val  A v1 = TPrim left_ty; type_of_val A v2 = TPrim right_ty\<rbrakk> \<Longrightarrow>
+ "\<lbrakk> binop_type bop = Some (targs, ret_ty); 
+    type_of_val  A v1 = TPrim left_ty; type_of_val A v2 = TPrim right_ty;
+   (left_ty, right_ty) \<in> targs \<rbrakk> \<Longrightarrow>
     \<exists>v. (binop_eval_val bop v1 v2) = Some v "
   by (cases bop; rule lit_val_elim[where v=v1]; rule lit_val_elim[where v=v2]; auto)
 
@@ -193,20 +195,16 @@ next
   moreover from this have "type_of_val A v' = TPrim arg_ty" using TypUnOp by auto
   ultimately show ?case using \<open>unop_type uop = (arg_ty, ret_ty)\<close> unop_type_correct by fastforce 
 next
-  case (TypBinOpMono bop left_ty right_ty ret_ty \<Delta> e1 e2)
+  case (TypBinOpMono bop targs ret_ty \<Delta> e1 left_ty e2 right_ty)
   from this obtain v1 v2 where 
      "A, \<Lambda>, \<Gamma>, \<Omega> \<turnstile> \<langle>e1, n_s\<rangle> \<Down> v1" and "A, \<Lambda>, \<Gamma>, \<Omega> \<turnstile> \<langle>e2, n_s\<rangle> \<Down> v2" and 
      E:"binop_eval_val bop v1 v2 = Some v"
     by auto
   moreover from this have T1:"type_of_val A v1 = TPrim left_ty" and 
     T2:"type_of_val A v2 = TPrim right_ty" using TypBinOpMono by auto
-  ultimately show ?case using \<open>binop_type bop = Some ((left_ty, right_ty), ret_ty)\<close> binop_type_correct by fastforce
-next
-  case (TypBinopRealDiv \<Delta> e1 t1 e2 t2)
-  from this obtain v1 v2 where "binop_eval_val RealDiv v1 v2 = Some v"
-    by auto
-  then show ?case using binop_realdiv_type_correct
-    by auto
+  ultimately show ?case using \<open>(left_ty, right_ty) \<in> targs\<close> \<open>binop_type bop = Some (targs, ret_ty)\<close> binop_type_correct      
+    using TypBinOpMono.hyps(2) 
+    by fastforce
 next
   case (TypBinopPoly bop \<Delta> e1 ty1 e2 ty2 ty_inst)
   from this obtain v1 v2 where 
@@ -366,7 +364,7 @@ next
   thus ?case using \<open>unop_type uop = (arg_ty, ret_ty)\<close> unop_progress RedE RedUnOp
     by (metis (full_types)) 
 next
-  case (TypBinOpMono bop left_ty right_ty ret_ty \<Delta> e1 e2)
+  case (TypBinOpMono bop targs ret_ty \<Delta> e1 left_ty e2 right_ty)
   have "\<exists>a. A,\<Lambda>,\<Gamma>,\<Omega> \<turnstile> \<langle>e1,n_s\<rangle> \<Down> a" 
     apply (rule TypBinOpMono.IH) using TypBinOpMono.prems by auto
   moreover have "\<exists>a. A,\<Lambda>,\<Gamma>,\<Omega> \<turnstile> \<langle>e2,n_s\<rangle> \<Down> a"
@@ -379,24 +377,8 @@ next
   moreover from RedRight have "type_of_val A v2 = TPrim right_ty"
     using TypBinOpMono.IH TypBinOpMono.prems preservation(1)[OF \<open>list_all closed \<Omega>\<close> TypBinOpMono.prems(5) TypBinOpMono.prems(6) TypBinOpMono.prems(7) Wf_\<Gamma> Wf_F]
     by fastforce
-  ultimately show ?case using \<open>binop_type bop = Some ((left_ty, right_ty), ret_ty)\<close> binop_progress RedBinOp
-    by (metis (no_types, lifting))
-next
-  case (TypBinopRealDiv \<Delta> e1 t1 e2 t2)
-    have "\<exists>a. A,\<Lambda>,\<Gamma>,\<Omega> \<turnstile> \<langle>e1,n_s\<rangle> \<Down> a" 
-    apply (rule TypBinopRealDiv.IH) using TypBinopRealDiv.prems by auto
-  moreover have "\<exists>a. A,\<Lambda>,\<Gamma>,\<Omega> \<turnstile> \<langle>e2,n_s\<rangle> \<Down> a"
-    apply (rule TypBinopRealDiv.IH) using TypBinopRealDiv.prems by auto
-  ultimately  obtain v1 v2 where RedLeft:"A,\<Lambda>,\<Gamma>,\<Omega> \<turnstile> \<langle>e1,n_s\<rangle> \<Down> v1" and  RedRight:"A,\<Lambda>,\<Gamma>,\<Omega> \<turnstile> \<langle>e2,n_s\<rangle> \<Down> v2"
-    by auto
-  moreover from RedLeft have "type_of_val A v1 = TPrim TReal \<or> type_of_val A v1 = TPrim TInt"      
-    using TypBinopRealDiv.prems TypBinopRealDiv.hyps preservation(1)[OF \<open>list_all closed \<Omega>\<close> TypBinopRealDiv.prems(5) TypBinopRealDiv.prems(6) TypBinopRealDiv.prems(7) Wf_\<Gamma> Wf_F \<open>F,\<Delta> \<turnstile> e1 : TPrim t1\<close>]
-    by auto    
-  moreover from RedRight have "type_of_val A v2 = TPrim TReal \<or> type_of_val A v2 = TPrim TInt"      
-    using TypBinopRealDiv.prems TypBinopRealDiv.hyps preservation(1)[OF \<open>list_all closed \<Omega>\<close> TypBinopRealDiv.prems(5) TypBinopRealDiv.prems(6) TypBinopRealDiv.prems(7) Wf_\<Gamma> Wf_F \<open>F,\<Delta> \<turnstile> e2 : TPrim t2\<close>]
-    by auto    
-  ultimately show ?case using RedBinOp binop_realdiv_progress
-    by metis   
+  ultimately show ?case using \<open>binop_type bop = Some (targs, ret_ty)\<close> \<open>(left_ty, right_ty) \<in> targs\<close> binop_progress RedBinOp
+    by metis
 next
   case (TypBinopPoly bop \<Delta> e1 ty1 e2 ty2 ty_inst)
   have "\<exists>a. A,\<Lambda>,\<Gamma>,\<Omega> \<turnstile> \<langle>e1,n_s\<rangle> \<Down> a" 
