BoogieLang/TypingML.thy
@@ -3,10 +3,9 @@ theory TypingML
 begin               
 
 ML \<open>
-fun assm_full_simp_solved_tac ctxt = (asm_full_simp_tac ctxt |> SOLVED')
 
 fun binop_mono_tac ctxt lookup_assms func_assms =
-  FIRST' [
+  FIRST' [  
   resolve_tac ctxt [@{thm TypVar}] THEN' (assm_full_simp_solved_tac (ctxt addsimps lookup_assms)),
   resolve_tac ctxt [@{thm TypBVar}] THEN' assm_full_simp_solved_tac ctxt,
   resolve_tac ctxt [@{thm TypPrim}] THEN' assm_full_simp_solved_tac ctxt,
@@ -31,31 +30,54 @@ fun binop_poly_tac ctxt hint_thm =
   resolve_tac ctxt ([@{thm typ_binop_poly_helper} OF [hint_thm]]) THEN'
   assm_full_simp_solved_tac ctxt
 
-fun simulate_tac tac st =
-  (case Seq.pull (tac st) of
-            NONE => NONE
-          | SOME (st', _) => SOME st')
+fun binop_poly_tac_no_hint ctxt =  
+  resolve_tac ctxt ([@{thm typ_binop_poly_helper_empty}]) THEN'
+  assm_full_simp_solved_tac ctxt
 
 (*
 hint_thms must provide the type substitutions as theorems (see TypingHelper.thy)
-for the equality operators, where the order is given from left to right
+for the equality operators, where the order is given from left to right.
+
+simulate_determ_tac is used to check whether a tactic succeeds (in which case typing_tac continues).
+Note that this tactic does not track how many subgoals were generated and still need to be solved from
+the initial subgoal. As a result, it is possible that the tactic solves a goal that was generated
+from the original subgoal. We might want to adjust that.
 *)
 fun typing_tac ctxt hint_thms lookup_assms func_assms i st =  
 let val simp_solve_continue = 
-   (case simulate_tac (assm_full_simp_solved_tac (ctxt addsimps [@{thm msubstT_opt_def}]) i) st of
+   (case simulate_determ_tac (assm_full_simp_solved_tac (ctxt addsimps [@{thm msubstT_opt_def}]) i) st of
       NONE => Seq.single st
     | SOME st' => typing_tac ctxt hint_thms lookup_assms func_assms i st'
    )
 in
-  (case simulate_tac (binop_mono_tac ctxt lookup_assms func_assms i) st of
+  (case simulate_determ_tac (binop_mono_tac ctxt lookup_assms func_assms i) st of
     NONE => 
       (case hint_thms of
          [] => simp_solve_continue
        | (hint :: hint_rest) => 
-         (case simulate_tac (binop_poly_tac ctxt hint i) st of
+         (case simulate_determ_tac (binop_poly_tac ctxt hint i) st of
             NONE => simp_solve_continue
           | SOME st' => typing_tac ctxt hint_rest lookup_assms func_assms i st'))
    | SOME st' => typing_tac ctxt hint_thms lookup_assms func_assms i st'
+  )
+end
+
+(* The following tactic is the same as typing_tac except where no hints are used for polymorphic 
+   binary operators (i.e., equality and inequality). This is useful in cases where the identity 
+   substitution is sufficient to type polymorphic binary operators. *)
+fun typing_tac_no_hints ctxt lookup_assms func_assms i st =  
+let val simp_solve_continue = 
+   (case simulate_determ_tac (assm_full_simp_solved_tac (ctxt addsimps [@{thm msubstT_opt_def}]) i) st of
+      NONE => Seq.single st
+    | SOME st' => typing_tac_no_hints ctxt lookup_assms func_assms i st'
+   )
+in
+  (case simulate_determ_tac (binop_mono_tac ctxt lookup_assms func_assms i) st of
+    NONE => 
+      (case simulate_determ_tac (binop_poly_tac_no_hint ctxt i) st of
+            NONE => simp_solve_continue
+          | SOME st' => typing_tac_no_hints ctxt  lookup_assms func_assms i st')
+   | SOME st' => typing_tac_no_hints ctxt lookup_assms func_assms i st'
   )
 end
 \<close>
